Got stuck!

rupicola/refinements2/Compiler.fst
@@ -10,8 +10,25 @@ open STLC
 (** Helpers to deal with Monotonicity of Pure **)
 module M = FStar.Monotonic.Pure
 
+let intro_pure_wp_monotonicity (#a:Type) (wp:pure_wp' a)
+  : Lemma
+      (requires M.is_monotonic wp)
+      (ensures pure_wp_monotonic a wp)
+    [SMTPat (pure_wp_monotonic a wp)]
+  = M.intro_pure_wp_monotonicity wp
+
 let pure_trivial #a : pure_wp a =
   fun p -> forall r. p r
+
+unfold let (<=) #a wp1 wp2 = pure_stronger a wp1 wp2
+unfold let ret #a x = pure_return a x
+
+unfold
+let helper_fapp wp (f:(x:'a -> PURE 'b (wp x))) (x:'a)
+  : Pure 'b (as_requires (wp x)) (as_ensures (wp x))
+  =
+  FStar.Monotonic.Pure.elim_pure_wp_monotonicity_forall ();
+  f x
 
 (** Typing environment **)
 type typsr = Type0
@@ -58,19 +75,28 @@ class compile_exp (#a:Type0) (g:env) (wpG:spec_env g a) (fs_e:fs_oexp g a wpG) =
 
 (** Just a helper typeclass **)
 unfold let compile_closed (#a:Type0) (s:a) =
-  compile_exp #a empty (fun _ -> s)
+  compile_exp #a empty (fun _ -> pure_trivial) (fun _ -> s)
 
-instance unit_elim #g : compile_exp g (fun _ -> ()) = {
-  e = EUnit;
-}
+instance unit_elim
+  #g
+  (#wpG:spec_env g unit)
+  (_:squash (forall fsG. wpG fsG <= ret ()))
+  : compile_exp g wpG (fun _ -> ())
+  = { e = EUnit; }
 
-instance true_elim #g : compile_exp g (fun _ -> true) = {
-  e = ETrue;
-}
+instance true_elim
+  #g
+  (#wpG:spec_env g bool)
+  (_:squash (forall fsG. wpG fsG <= ret true))
+  : compile_exp g wpG (fun _ -> true)
+  = { e = ETrue; }
 
-instance false_elim #g : compile_exp g (fun _ -> false) = {
-  e = EFalse;
-}
+instance false_elim
+  #g
+  (#wpG:spec_env g bool)
+  (_:squash (forall fsG. wpG fsG <= ret false))
+  : compile_exp g wpG (fun _ -> false)
+  = { e = EFalse; }
 
 let test_unit : compile_closed () = solve
 let test_true : compile_closed true = solve
@@ -85,50 +111,78 @@ let get_v' #g fsG i a =
 instance var_elim
   (#g:env)
   (a:Type)
+  (#wpG:spec_env g a)
   (x:var{Some? (g x) /\ a == Some?.v (g x)})
-  : compile_exp #a g (fun fsG -> get_v' fsG x a) = {
-    e = EVar x;
-}
+  (_:squash (forall fsG. wpG fsG <= ret (get_v' fsG x a)))
+  : compile_exp #a g wpG (fun fsG -> get_v' fsG x a)
+  = { e = EVar x; }
 
-let test1_var : compile_exp (extend unit empty) (fun fsG -> get_v' fsG 0 unit) = solve
+let test1_var
+  : compile_exp (extend unit empty) (fun _ -> pure_trivial) (fun fsG -> get_v' fsG 0 unit)
+  = solve
 
 instance var_elim_shrink1 (** CA: how to make this general? **)
   (g':env)
   (a:Type)
+  (#wpG:spec_env g' a)
   (t:typsr)
   (g:env{g' == extend t g})
   (x:var{Some? (g x) /\ a == Some?.v (g x)})
-  {| ce:compile_exp g' (fun fsG -> get_v' #g' fsG (x+1) a) |} (** this is not necessary. I am hoping that it can be modified to be recursive **)
-  : compile_exp g' (fun (fsG:fs_env g') -> get_v' #g (fs_shrink #t #g fsG) x a) = {
-    e = ce.e;
-  }
+  (_:squash (forall fsG. wpG fsG <= ret (get_v' fsG (x+1) a)))
+  {| ce:compile_exp g' wpG (fun fsG -> get_v' #g' fsG (x+1) a) |} (** this is not necessary. I am hoping that it can be modified to be recursive **)
+  (_:squash (forall fsG. wpG fsG <= ret (get_v' #g (fs_shrink #t fsG) x a)))
+  : compile_exp g' wpG (fun fsG -> get_v' #g (fs_shrink #t fsG) x a)
+  = { e = ce.e; }
 
 instance var_elim_shrink2 (** CA: how to make this general? **)
   (g':env)
   (a:Type)
+  (#wpG:spec_env g' a)
   (t1 t2:typsr)
   (g:env{g' == extend t1 (extend t2 g)})
   (x:var{Some? (g x) /\ a == Some?.v (g x)})
-  {| ce:compile_exp g' (fun fsG -> get_v' #g' fsG (x+2) a) |} (** this is not necessary. I am hoping that it can be modified to be recursive **)
-  : compile_exp g' (fun (fsG:fs_env g') -> get_v' #g (fs_shrink #t2 (fs_shrink #t1 fsG)) x a) = {
+  (_:squash (forall fsG. wpG fsG <= ret (get_v' fsG (x+2) a)))
+  {| ce:compile_exp g' wpG (fun fsG -> get_v' #g' fsG (x+2) a) |} (** this is not necessary. I am hoping that it can be modified to be recursive **)
+  (_:squash (forall fsG. wpG fsG <= ret (get_v' #g (fs_shrink #t2 (fs_shrink #t1 fsG)) x a)))
+  : compile_exp g' wpG (fun fsG -> get_v' #g (fs_shrink #t2 (fs_shrink #t1 fsG)) x a) = {
     e = ce.e;
   }
 
-let test2_var : compile_exp (extend unit (extend unit empty)) (fun fsG -> get_v' (fs_shrink fsG) 0 unit) =
-  solve
+let test2_var
+  : compile_exp (extend unit (extend unit empty)) (fun _ -> pure_trivial) (fun fsG -> get_v' (fs_shrink fsG) 0 unit)
+  = solve
 
-let test3_var : compile_exp (extend unit (extend unit (extend unit empty))) (fun fsG -> get_v' (fs_shrink (fs_shrink fsG)) 0 unit) =
-  solve
+let test3_var
+  : compile_exp (extend unit (extend unit (extend unit empty))) (fun _ -> pure_trivial) (fun fsG -> get_v' (fs_shrink (fs_shrink fsG)) 0 unit)
+  = solve
 
-instance lambda_elim
+let body_wp
+  #g
+  (#a:Type)
+  (#b:Type)
+  (#wpG:spec_env g (a -> b))
+  (f:fs_oexp g (a -> b) wpG)
+  : spec_env (extend a g) b
+  = fun fsG ->
+    let wp = fun p -> as_requires (wpG (fs_shrink #a fsG)) /\ forall r. (as_ensures (wpG (fs_shrink #a fsG)) (f (fs_shrink #a fsG))) ==> p r in
+    wp
+
+//   (fun fsG -> admit (); fun p -> wpG (fs_shrink #a fsG) (fun f' -> p (f' (get_v' fsG 0 a))))
+
+let lambda_elim
   #g
   (a:Type)
   (b:Type)
-  (f:fs_oexp g (a -> b))
-  {| cf: compile_exp #b (extend a g) (fun fsG -> f (fs_shrink #a fsG) (get_v' fsG 0 a)) |}
-  : compile_exp g f = {
-  e = ELam cf.e;
-}
+  (#wpG:spec_env g (a -> b))
+  (f:fs_oexp g (a -> b) wpG)
+  (_:squash (forall fsG. wpG fsG <= ret (f fsG)))
+  {| cf: compile_exp #b
+           (extend a g)
+           (body_wp f)
+           (fun fsG -> f (fs_shrink #a fsG) (get_v' fsG 0 a)) |}
+  : compile_exp #(a -> b) g wpG (fun fsG -> admit (); f fsG)
+  by (tadmit ())
+  = { e = ELam cf.e; }
 
 let test1_exp : compile_closed (fun (x:unit) -> ()) = solve
 let _ = assert (test1_exp.e == ELam (EUnit))
